FormalSystems/Preliminaries/NonEmptyList.lean
@@ -1,3 +1,0 @@
-/--Define the non-empty lists as a type.-/
-class NonEmptyList (α : Type u) extends (List α) where
-  nonEmpty : α.length > 0
